<?xml version="1.0"?>
<rdf:RDF xmlns="https://github.com/biotea/biotea-ontololgy/bioteaOnto#"
     xml:base="https://github.com/biotea/biotea-ontololgy/bioteaOnto"
     xmlns:pav="http://purl.org/pav/"
     xmlns:rdf="http://www.w3.org/1999/02/22-rdf-syntax-ns#"
     xmlns:owl="http://www.w3.org/2002/07/owl#"
     xmlns:xml="http://www.w3.org/XML/1998/namespace"
     xmlns:xsd="http://www.w3.org/2001/XMLSchema#"
     xmlns:rdfs="http://www.w3.org/2000/01/rdf-schema#"
     xmlns:biotea="https://github.com/biotea/biotea-ontololgy/bioteaOnto#">
    <owl:Ontology rdf:about="https://github.com/biotea/biotea-ontololgy/bioteaOnto">
        <rdfs:comment>An ontology to support the RDFization of scientific documents in the Biotea project</rdfs:comment>
    </owl:Ontology>
    


    <!-- 
    ///////////////////////////////////////////////////////////////////////////////////////
    //
    // Object Properties
    //
    ///////////////////////////////////////////////////////////////////////////////////////
     -->

    


    <!-- https://github.com/biotea/biotea-ontololgy/bioteaOnto#annotator -->

    <owl:ObjectProperty rdf:about="https://github.com/biotea/biotea-ontololgy/bioteaOnto#annotator">
        <rdfs:comment>Points to the annotator used to generate the semantic annotations in a document.</rdfs:comment>
    </owl:ObjectProperty>
    


    <!-- https://github.com/biotea/biotea-ontololgy/bioteaOnto#hasModel -->

    <owl:ObjectProperty rdf:about="https://github.com/biotea/biotea-ontololgy/bioteaOnto#hasModel">
        <rdfs:range rdf:resource="https://github.com/biotea/biotea-ontololgy/bioteaOnto#Model"/>
        <rdfs:comment>Points to the model used for the group-based distribution or group-narrowed semantic similarity.</rdfs:comment>
    </owl:ObjectProperty>
    


    <!-- https://github.com/biotea/biotea-ontololgy/bioteaOnto#hasTopic -->

    <owl:ObjectProperty rdf:about="https://github.com/biotea/biotea-ontololgy/bioteaOnto#hasTopic">
        <rdfs:range rdf:resource="https://github.com/biotea/biotea-ontololgy/bioteaOnto#Topic"/>
        <rdfs:comment>Points to the group with an assigend score (i.e., topic) in a group-based distribution.</rdfs:comment>
    </owl:ObjectProperty>
    


    <!-- https://github.com/biotea/biotea-ontololgy/bioteaOnto#link -->

    <owl:ObjectProperty rdf:about="https://github.com/biotea/biotea-ontololgy/bioteaOnto#link">
        <rdfs:domain rdf:resource="https://github.com/biotea/biotea-ontololgy/bioteaOnto#Biolink"/>
        <rdfs:comment>Link between a biotea:Biolink and a semantic annotation. Used to record the semantic annotations participating in the similarity between two documents.</rdfs:comment>
    </owl:ObjectProperty>
    


    <!-- https://github.com/biotea/biotea-ontololgy/bioteaOnto#onDocument -->

    <owl:ObjectProperty rdf:about="https://github.com/biotea/biotea-ontololgy/bioteaOnto#onDocument">
        <rdfs:domain rdf:resource="https://github.com/biotea/biotea-ontololgy/bioteaOnto#TopicDistribution"/>
        <rdfs:comment>Points to the document for which the group-based distribution has been calculated.</rdfs:comment>
    </owl:ObjectProperty>
    


    <!-- https://github.com/biotea/biotea-ontololgy/bioteaOnto#onQueryDocument -->

    <owl:ObjectProperty rdf:about="https://github.com/biotea/biotea-ontololgy/bioteaOnto#onQueryDocument">
        <rdfs:domain rdf:resource="https://github.com/biotea/biotea-ontololgy/bioteaOnto#Biolink"/>
        <rdfs:comment>Points to the query document used to calculate a semantic similarity.</rdfs:comment>
    </owl:ObjectProperty>
    


    <!-- https://github.com/biotea/biotea-ontololgy/bioteaOnto#onRelatedDocument -->

    <owl:ObjectProperty rdf:about="https://github.com/biotea/biotea-ontololgy/bioteaOnto#onRelatedDocument">
        <rdfs:domain rdf:resource="https://github.com/biotea/biotea-ontololgy/bioteaOnto#Biolink"/>
        <rdfs:comment>Points to the compared document used to calculate a semantic similarity.</rdfs:comment>
    </owl:ObjectProperty>
    


    <!-- 
    ///////////////////////////////////////////////////////////////////////////////////////
    //
    // Data properties
    //
    ///////////////////////////////////////////////////////////////////////////////////////
     -->

    


    <!-- https://github.com/biotea/biotea-ontololgy/bioteaOnto#group -->

    <owl:DatatypeProperty rdf:about="https://github.com/biotea/biotea-ontololgy/bioteaOnto#group">
        <rdfs:range rdf:resource="http://www.w3.org/2001/XMLSchema#string"/>
        <rdfs:comment>Name given to a semantic group in a Model.</rdfs:comment>
    </owl:DatatypeProperty>
    


    <!-- https://github.com/biotea/biotea-ontololgy/bioteaOnto#idf -->

    <owl:DatatypeProperty rdf:about="https://github.com/biotea/biotea-ontololgy/bioteaOnto#idf">
        <rdfs:range rdf:resource="http://www.w3.org/2001/XMLSchema#double"/>
        <rdfs:comment>Inverse document frequency of a term in a collection of documents.</rdfs:comment>
    </owl:DatatypeProperty>
    


    <!-- https://github.com/biotea/biotea-ontololgy/bioteaOnto#occurrences -->

    <owl:DatatypeProperty rdf:about="https://github.com/biotea/biotea-ontololgy/bioteaOnto#occurrences">
        <owl:equivalentProperty rdf:resource="https://github.com/biotea/biotea-ontololgy/bioteaOnto#tf"/>
        <rdfs:range rdf:resource="http://www.w3.org/2001/XMLSchema#integer"/>
        <rdfs:comment>Legacy, see biotea:tf.</rdfs:comment>
    </owl:DatatypeProperty>
    


    <!-- https://github.com/biotea/biotea-ontololgy/bioteaOnto#score -->

    <owl:DatatypeProperty rdf:about="https://github.com/biotea/biotea-ontololgy/bioteaOnto#score">
        <rdfs:range rdf:resource="http://www.w3.org/2001/XMLSchema#double"/>
        <rdfs:comment>Distribution or similarity score.</rdfs:comment>
    </owl:DatatypeProperty>
    


    <!-- https://github.com/biotea/biotea-ontololgy/bioteaOnto#tf -->

    <owl:DatatypeProperty rdf:about="https://github.com/biotea/biotea-ontololgy/bioteaOnto#tf">
        <rdfs:range rdf:resource="http://www.w3.org/2001/XMLSchema#integer"/>
        <rdfs:comment>Term frequency of a term in a document.</rdfs:comment>
    </owl:DatatypeProperty>
    


    <!-- https://github.com/biotea/biotea-ontololgy/bioteaOnto#totalTF -->

    <owl:DatatypeProperty rdf:about="https://github.com/biotea/biotea-ontololgy/bioteaOnto#totalTF">
        <rdfs:domain rdf:resource="https://github.com/biotea/biotea-ontololgy/bioteaOnto#TopicDistribution"/>
        <rdfs:range rdf:resource="http://www.w3.org/2001/XMLSchema#integer"/>
        <rdfs:comment>Total term frequency of all the terms used to calculate a TopicDistribution.</rdfs:comment>
    </owl:DatatypeProperty>
    


    <!-- 
    ///////////////////////////////////////////////////////////////////////////////////////
    //
    // Classes
    //
    ///////////////////////////////////////////////////////////////////////////////////////
     -->

    


    <!-- https://github.com/biotea/biotea-ontololgy/bioteaOnto#Biolink -->

    <owl:Class rdf:about="https://github.com/biotea/biotea-ontololgy/bioteaOnto#Biolink">
        <rdfs:comment>Semantic similarity between a query document and a related document. A score [0.0, 1.0] is assigned to the similarity. The similarity can be restricted to a set of groups defined in a model (e.g. Biolinks or UMLS semantic groups). The semantic annotations participating in the similarity are also recorded (optional).</rdfs:comment>
    </owl:Class>
    


    <!-- https://github.com/biotea/biotea-ontololgy/bioteaOnto#Model -->

    <owl:Class rdf:about="https://github.com/biotea/biotea-ontololgy/bioteaOnto#Model">
        <rdfs:comment>A model of semantic groups, e.g., UMLS or Biolinks semantic groups. A set of concepts is associated to one group and only one in the model.</rdfs:comment>
    </owl:Class>
    


    <!-- https://github.com/biotea/biotea-ontololgy/bioteaOnto#SemanticAnnotation -->

    <owl:Class rdf:about="https://github.com/biotea/biotea-ontololgy/bioteaOnto#SemanticAnnotation">
        <rdfs:comment>A portion of a document (i.e., word or sequence of words) associated to a semantic entity (e.g., CUI in UMLS).</rdfs:comment>
    </owl:Class>
    


    <!-- https://github.com/biotea/biotea-ontololgy/bioteaOnto#Topic -->

    <owl:Class rdf:about="https://github.com/biotea/biotea-ontololgy/bioteaOnto#Topic">
        <rdfs:comment>Group name and distribution score calculated for such a group.</rdfs:comment>
    </owl:Class>
    


    <!-- https://github.com/biotea/biotea-ontololgy/bioteaOnto#TopicDistribution -->

    <owl:Class rdf:about="https://github.com/biotea/biotea-ontololgy/bioteaOnto#TopicDistribution">
        <rdfs:comment>A class representing a Biolinks group-based distribution. Such a distribution is defined on a document and all Biolinks group. A score is associated to each group, representing the weight of that group in the document.</rdfs:comment>
    </owl:Class>
</rdf:RDF>



<!-- Generated by the OWL API (version 4.2.5.20160517-0735) https://github.com/owlcs/owlapi -->

